src/proof/pure_objects.v
@@ -795,6 +795,84 @@ Qed.
 End proof.
 End KObjectV.
 
+Module PreconditionsV.
+Section def.
+Context `{hG: !heapGS Σ}.
+Record t := mk {
+  UID' : option types.UID.t;
+  ResourceVersion' : option go_string;
+}.
+
+Definition deepown (c: v1.Preconditions.t) (v: t) dq: iProp Σ :=
+  "%Hdeepown_uid_none" ∷ ⌜ c.(v1.Preconditions.UID') = null ↔ v.(UID') = None⌝ ∗
+  "Hdeepown_uid_some" ∷ (match v.(UID') with
+  | Some vu => ∃ cu, c.(v1.Preconditions.UID') ↦{dq} cu ∗ ⌜ cu = vu ⌝
+  | None => True%I
+  end) ∗
+  "%Hdeepown_resourceversion_none" ∷ ⌜ c.(v1.Preconditions.ResourceVersion') = null ↔ v.(ResourceVersion') = None⌝ ∗
+  "Hdeepown_resourceversion_some" ∷ (match v.(ResourceVersion') with
+  | Some vrv => ∃ crv, c.(v1.Preconditions.ResourceVersion') ↦{dq} crv ∗ ⌜ crv = vrv ⌝
+  | None => True%I
+  end).
+
+Definition deepown_l l v dq: iProp Σ :=
+  ∃ c, l ↦{dq} c ∗ deepown c v dq.
+
+Definition valid_interface i (l : loc) : Prop :=
+  i = interface.mk (ptrT.id v1.Preconditions.id) #l.
+
+Definition deepown_i i v dq: iProp Σ :=
+  ∃ l, ⌜ valid_interface i l ⌝ ∗ deepown_l l v dq.
+End def.
+End PreconditionsV.
+
+Module DeleteOptionsV.
+Section def.
+Context `{hG: !heapGS Σ}.
+Record t := mk {
+  TypeMeta' : v1.TypeMeta.t;
+  GracePeriodSeconds' : option w64;
+  Preconditions' : option PreconditionsV.t;
+  OrphanDependents' : option bool;
+  PropagationPolicy' : option go_string;
+  (* DryRun' : slice.t; *)
+  (* IgnoreStoreReadErrorWithClusterBreakingPotential' : loc; *)
+}.
+
+Definition deepown (c: v1.DeleteOptions.t) (v: t) dq: iProp Σ :=
+  "%Hdeepown_typemeta" ∷ ⌜ c.(v1.DeleteOptions.TypeMeta') = v.(TypeMeta') ⌝ ∗
+  "%Hdeepown_graceperiodseconds_none" ∷ ⌜ c.(v1.DeleteOptions.GracePeriodSeconds') = null ↔ v.(GracePeriodSeconds') = None⌝ ∗
+  "Hdeepown_graceperiodseconds_some" ∷ (match v.(GracePeriodSeconds') with
+  | Some vgps => ∃ cgps, c.(v1.DeleteOptions.GracePeriodSeconds') ↦{dq} cgps ∗ ⌜ cgps = vgps ⌝
+  | None => True%I
+  end) ∗
+  "%Hdeepown_preconditions_none" ∷ ⌜ c.(v1.DeleteOptions.Preconditions') = null ↔ v.(Preconditions') = None⌝ ∗
+  "Hdeepown_preconditions_some" ∷ (match v.(Preconditions') with
+  | Some vp => ∃ cp, c.(v1.DeleteOptions.Preconditions') ↦{dq} cp ∗ PreconditionsV.deepown cp vp dq
+  | None => True%I
+  end) ∗
+  "%Hdeepown_orphandependents_none" ∷ ⌜ c.(v1.DeleteOptions.OrphanDependents') = null ↔ v.(OrphanDependents') = None⌝ ∗
+  "Hdeepown_orphandependents_some" ∷ (match v.(OrphanDependents') with
+  | Some vod => ∃ cod, c.(v1.DeleteOptions.OrphanDependents') ↦{dq} cod ∗ ⌜ cod = vod ⌝
+  | None => True%I
+  end) ∗
+  "%Hdeepown_propagationpolicy_none" ∷ ⌜ c.(v1.DeleteOptions.PropagationPolicy') = null ↔ v.(PropagationPolicy') = None⌝ ∗
+  "Hdeepown_propagationpolicy_some" ∷ (match v.(PropagationPolicy') with
+  | Some vpp => ∃ cpp, c.(v1.DeleteOptions.PropagationPolicy') ↦{dq} cpp ∗ ⌜ cpp = vpp ⌝
+  | None => True%I
+  end).
+
+Definition deepown_l l v dq: iProp Σ :=
+  ∃ c, l ↦{dq} c ∗ deepown c v dq.
+
+Definition valid_interface i (l : loc) : Prop :=
+  i = interface.mk (ptrT.id v1.DeleteOptions.id) #l.
+
+Definition deepown_i i v dq: iProp Σ :=
+  ∃ l, ⌜ valid_interface i l ⌝ ∗ deepown_l l v dq.
+End def.
+End DeleteOptionsV.
+
 Global Instance key_eq_dec : EqDecision KKey.t.
 Proof. solve_decision. Qed.
   
